theories/refinements/static_gradual/help_left.v
@@ -10,7 +10,7 @@ From fae_gtlc_mu.cast_calculus Require Export consistency.structural.definition.
 From fae_gtlc_mu.backtranslation Require Export cast_help.general cast_help.extract cast_help.embed.
 
 Section extract_embed.
-  Context `{!heapG Σ,!gradRN Σ}.
+  Context `{!implG Σ,!specG Σ}.
   Notation D := (prodO stlc_mu.lang.valO cast_calculus.lang.valO -n> iPropO Σ).
   (* Implicit Types e : stlc_mu.lang.expr. *)
   (* Implicit Types e : stlc_mu.lang.expr. *)
